contrib/subtac/subtac_command.ml
@@ -57,7 +57,7 @@ let interp_gen kind isevars env
                c =
   let c' = Constrintern.intern_gen (kind=IsType) ~impls ~allow_soapp ~ltacvars (Evd.evars_of !isevars) env c in
   let c' = Subtac_utils.rewrite_cases env c' in
-    (try trace (str "Pretyping " ++ my_print_constr_expr c) with _ -> ());
+(*     (try trace (str "Pretyping " ++ my_print_constr_expr c) with _ -> ()); *)
   let c' = SPretyping.pretype_gen isevars env ([],[]) kind c' in
     evar_nf isevars c'
     
@@ -150,14 +150,6 @@ let collect_non_rec env =
   in 
   searchrec [] 
 
-
-let filter_map f l = 
-  let rec aux acc = function
-      hd :: tl -> (match f hd with Some t -> aux (t :: acc) tl
-		     | None -> aux acc tl)
-    | [] -> List.rev acc
-  in aux [] l
-
 let list_of_local_binders l = 
   let rec aux acc = function
       Topconstr.LocalRawDef (n, c) :: tl -> aux ((n, Some c, None) :: acc) tl
@@ -176,25 +168,29 @@ let rec gen_rels = function
     0 -> []
   | n -> mkRel n :: gen_rels (pred n)
 
+let split_args n rel = match list_chop ((List.length rel) - n) rel with
+    (l1, x :: l2) -> l1, x, l2
+  | _ -> assert(false)
+
 let build_wellfounded (recname, n, bl,arityc,body) r measure notation boxed =
   let sigma = Evd.empty in
   let isevars = ref (Evd.create_evar_defs sigma) in
   let env = Global.env() in 
-  let pr c = my_print_constr env c in
-  let prr = Printer.pr_rel_context env in
-  let prn = Printer.pr_named_context env in
-  let pr_rel env = Printer.pr_rel_context env in
   let nc = named_context env in
   let nc_len = named_context_length nc in
-  let _ = 
-    try debug 2 (str "In named context: " ++ prn (named_context env) ++ str "Rewriting fixpoint: " ++ Ppconstr.pr_id recname ++ 
-		 Ppconstr.pr_binders bl ++ str " : " ++ 
-		 Ppconstr.pr_constr_expr arityc ++ str " := " ++ spc () ++
-		 Ppconstr.pr_constr_expr body)
-    with _ -> ()
-  in
+(*   let pr c = my_print_constr env c in *)
+(*   let prr = Printer.pr_rel_context env in *)
+(*   let prn = Printer.pr_named_context env in *)
+(*   let pr_rel env = Printer.pr_rel_context env in *)
+(*   let _ =  *)
+(*     try debug 2 (str "In named context: " ++ prn (named_context env) ++ str "Rewriting fixpoint: " ++ Ppconstr.pr_id recname ++  *)
+(* 		 Ppconstr.pr_binders bl ++ str " : " ++  *)
+(* 		 Ppconstr.pr_constr_expr arityc ++ str " := " ++ spc () ++ *)
+(* 		 Ppconstr.pr_constr_expr body) *)
+(*     with _ -> () *)
+    (*   in *)
   let env', binders_rel = interp_context isevars env bl in
-  let after, ((argname, _, argtyp) as arg), before = list_chop_hd (succ n) binders_rel in
+  let after, ((argname, _, argtyp) as arg), before = split_args (succ n) binders_rel in
   let before_length, after_length = List.length before, List.length after in
   let argid = match argname with Name n -> n | _ -> assert(false) in
   let _liftafter = lift_binders 1 after_length after in
@@ -226,15 +222,14 @@ let build_wellfounded (recname, n, bl,arityc,body) r measure notation boxed =
   in
   let argid' = id_of_string (string_of_id argid ^ "'") in
   let wfarg len = (Name argid', None, 
-  		   mkSubset (Name argid') argtyp 
+  		   mkSubset (Name argid') (lift len argtyp) 
 		     (wf_rel_fun (mkRel 1) (mkRel (len + 1))))
   in
   let top_bl = after @ (arg :: before) in
   let intern_bl = after @ (wfarg 1 :: arg :: before) in
   let top_env = push_rel_context top_bl env in
-  let intern_env = push_rel_context intern_bl env in
+  let _intern_env = push_rel_context intern_bl env in
   let top_arity = interp_type isevars top_env arityc in
-  (try debug 2 (str "Intern bl: " ++ prr intern_bl) with _ -> ());
   let proj = (Lazy.force sig_).Coqlib.proj1 in
   let projection = 
     mkApp (proj, [| argtyp ;
@@ -243,32 +238,32 @@ let build_wellfounded (recname, n, bl,arityc,body) r measure notation boxed =
 		    mkRel 1
 		 |])
   in
-  (try debug 2 (str "Top arity: " ++ my_print_constr top_env top_arity) with _ -> ());
+    (*   (try debug 2 (str "Top arity: " ++ my_print_constr top_env top_arity) with _ -> ()); *)
   let intern_arity = substnl [projection] after_length top_arity in 
-  (try debug 2 (str "Top arity after subst: " ++ my_print_constr intern_env intern_arity) with _ -> ());
+(*   (try debug 2 (str "Top arity after subst: " ++ my_print_constr intern_env intern_arity) with _ -> ()); *)
   let intern_before_env = push_rel_context before env in
   let intern_fun_bl = after @ [wfarg 1]  in
-  (try debug 2 (str "Intern fun bl: " ++ prr intern_fun_bl) with _ -> ());
+(*   (try debug 2 (str "Intern fun bl: " ++ prr intern_fun_bl) with _ -> ()); *)
   let intern_fun_arity = intern_arity in
-  (try debug 2 (str "Intern fun arity: " ++ 
-		  my_print_constr intern_env intern_fun_arity) with _ -> ());
+(*   (try debug 2 (str "Intern fun arity: " ++  *)
+(* 		  my_print_constr intern_env intern_fun_arity) with _ -> ()); *)
   let intern_fun_arity_prod = it_mkProd_or_LetIn intern_fun_arity intern_fun_bl in
   let intern_fun_binder = (Name recname, None, intern_fun_arity_prod) in
   let fun_bl = after @ (intern_fun_binder :: [arg]) in
-  (try debug 2 (str "Fun bl: " ++ pr_rel intern_before_env fun_bl ++ spc ()) with _ -> ());
+(*   (try debug 2 (str "Fun bl: " ++ pr_rel intern_before_env fun_bl ++ spc ()) with _ -> ()); *)
   let fun_env = push_rel_context fun_bl intern_before_env in
   let fun_arity = interp_type isevars fun_env arityc in
   let intern_body = interp_casted_constr isevars fun_env body fun_arity in
   let intern_body_lam = it_mkLambda_or_LetIn intern_body fun_bl in
-  let _ = 
-      try debug 2 (str "Fun bl: " ++ prr fun_bl ++ spc () ++
-		   str "Intern bl" ++ prr intern_bl ++ spc () ++
-		   str "Top bl" ++ prr top_bl ++ spc () ++
-		   str "Intern arity: " ++ pr intern_arity ++
-		   str "Top arity: " ++ pr top_arity ++ spc () ++
-		   str "Intern body " ++ pr intern_body_lam)
-      with _ -> ()
-  in
+(*   let _ =  *)
+(*       try debug 2 (str "Fun bl: " ++ prr fun_bl ++ spc () ++ *)
+(* 		   str "Intern bl" ++ prr intern_bl ++ spc () ++ *)
+(* 		   str "Top bl" ++ prr top_bl ++ spc () ++ *)
+(* 		   str "Intern arity: " ++ pr intern_arity ++ *)
+(* 		   str "Top arity: " ++ pr top_arity ++ spc () ++ *)
+(* 		   str "Intern body " ++ pr intern_body_lam) *)
+(*       with _ -> () *)
+(*   in *)
   let _impl = 
     if Impargs.is_implicit_args()
     then Impargs.compute_implicits top_env top_arity
@@ -292,53 +287,48 @@ let build_wellfounded (recname, n, bl,arityc,body) r measure notation boxed =
   let def_appl = applist (fix_def, gen_rels (after_length + 1)) in
   let def = it_mkLambda_or_LetIn def_appl binders_rel in
   let typ = it_mkProd_or_LetIn top_arity binders_rel in
-    debug 2 (str "Constructed def");
-    debug 2 (my_print_constr intern_before_env def);
-    debug 2 (str "Type: " ++ my_print_constr env typ);
   let fullcoqc = Evarutil.nf_isevar !isevars def in
   let fullctyp = Evarutil.nf_isevar !isevars typ in
-  let _ = try trace (str "After evar normalization: " ++ spc () ++
-		 str "Coq term: " ++ my_print_constr env fullcoqc ++ spc ()
-		     ++ str "Coq type: " ++ my_print_constr env fullctyp) 
-     with _ -> () 
-  in
+(*   let _ = try trace (str "After evar normalization: " ++ spc () ++ *)
+(* 		 str "Coq term: " ++ my_print_constr env fullcoqc ++ spc () *)
+(* 		     ++ str "Coq type: " ++ my_print_constr env fullctyp)  *)
+(*      with _ -> ()  *)
+(*   in *)
   let evm = non_instanciated_map env isevars in
-  let _ = try trace (str "Non instanciated evars map: " ++ Evd.pr_evar_map evm)  with _ -> () in
+    (*   let _ = try trace (str "Non instanciated evars map: " ++ Evd.pr_evar_map evm)  with _ -> () in *)
   let evars, evars_def = Eterm.eterm_obligations recname nc_len evm fullcoqc (Some fullctyp) in
-    (try trace (str "Generated obligations : ");
-       Array.iter
-	 (fun (n, t, _) -> trace (str "Evar " ++ str (string_of_id n) ++ spc () ++ my_print_constr env t))
-	 evars;
-     with _ -> ());    
-      trace (str "Adding to obligations list");
-      Subtac_obligations.add_entry recname evars_def fullctyp evars;
-      trace (str "Added to obligations list")
-(*
+    (*     (try trace (str "Generated obligations : "); *)
+(*        Array.iter *)
+    (* 	 (fun (n, t, _) -> trace (str "Evar " ++ str (string_of_id n) ++ spc () ++ my_print_constr env t)) *)
+    (* 	 evars; *)
+    (*      with _ -> ());     *)
+    Subtac_obligations.add_definition recname evars_def fullctyp evars
+    
 let build_mutrec l boxed = 
-  let sigma = Evd.empty
-  and env0 = Global.env()
-  in 
+  let sigma = Evd.empty and env = Global.env () in 
+  let nc = named_context env in
+  let nc_len = named_context_length nc in
   let lnameargsardef =
-    (*List.map (fun (f, d) -> Subtac_interp_fixpoint.rewrite_fixpoint env0 protos (f, d))*)
+    (*List.map (fun (f, d) -> Subtac_interp_fixpoint.rewrite_fixpoint env protos (f, d))*)
     l
   in
   let lrecnames = List.map (fun ((f,_,_,_,_),_) -> f) lnameargsardef 
   and nv = List.map (fun ((_,n,_,_,_),_) -> n) lnameargsardef
   in
     (* Build the recursive context and notations for the recursive types *)
-  let (rec_sign,rec_impls,arityl) = 
+  let (rec_sign,rec_env,rec_impls,arityl) = 
     List.fold_left 
-      (fun (env,impls,arl) ((recname, n, bl,arityc,body),_) -> 
+      (fun (sign,env,impls,arl) ((recname, n, bl,arityc,body),_) -> 
 	 let isevars = ref (Evd.create_evar_defs sigma) in	  
 	 let arityc = Command.generalize_constr_expr arityc bl in
-	 let arity = interp_type isevars env0 arityc in
+	 let arity = interp_type isevars env arityc in
 	 let impl = 
 	   if Impargs.is_implicit_args()
-	   then Impargs.compute_implicits env0 arity
+	   then Impargs.compute_implicits env arity
 	   else [] in
 	 let impls' =(recname,([],impl,compute_arguments_scope arity))::impls in
-	   (Environ.push_named (recname,None,arity) env, impls', (isevars, None, arity)::arl))
-      (env0,[],[]) lnameargsardef in
+	   ((recname,None,arity) :: sign, Environ.push_named (recname,None,arity) env, impls', (isevars, None, arity)::arl))
+      ([],env,[],[]) lnameargsardef in
   let arityl = List.rev arityl in
   let notations = 
     List.fold_right (fun (_,ntnopt) l -> option_cons ntnopt l) 
@@ -357,11 +347,11 @@ let build_mutrec l boxed =
 	     match info with
 		 None ->
 		   let def = abstract_constr_expr def bl in
-		     isevars, info, interp_casted_constr isevars rec_sign ~impls:([],rec_impls)
+		     isevars, info, interp_casted_constr isevars rec_env ~impls:([],rec_impls)
 		       def arity
 	       | Some (n, artyp, wfrel, fun_bl, intern_bl, intern_arity) ->
-		   let rec_sign = push_rel_context fun_bl rec_sign in
-		   let cstr = interp_casted_constr isevars rec_sign ~impls:([],rec_impls)
+		   let rec_env = push_rel_context fun_bl rec_env in
+		   let cstr = interp_casted_constr isevars rec_env ~impls:([],rec_impls)
 				def intern_arity
 		   in isevars, info, it_mkLambda_or_LetIn cstr fun_bl)
           lnameargsardef arityl
@@ -369,162 +359,33 @@ let build_mutrec l boxed =
 	States.unfreeze fs; raise e in
     States.unfreeze fs; def 
   in
-
   let (lnonrec,(namerec,defrec,arrec,nvrec)) = 
-    collect_non_rec env0 lrecnames recdef arityl nv in
-  let declare arrec defrec =
-    let recvec = 
-      Array.map (subst_vars (List.rev (Array.to_list namerec))) defrec in
-    let recdecls = (Array.map (fun id -> Name id) namerec, arrec, recvec) in
-    let rec declare i fi =
-      (try trace (str "Declaring: " ++ pr_id fi ++ spc () ++
-		  my_print_constr env0 (recvec.(i)));
-       with _ -> ());
-      let ce = 
-	{ const_entry_body = mkFix ((nvrec,i),recdecls); 
-          const_entry_type = Some arrec.(i);
-          const_entry_opaque = false;
-          const_entry_boxed = boxed} in
-      let kn = Declare.declare_constant fi (DefinitionEntry ce,IsDefinition Fixpoint)
-      in (ConstRef kn)
-    in 
-      (* declare the recursive definitions *)
-    let lrefrec = Array.mapi declare namerec in
-      Options.if_verbose ppnl (recursive_message lrefrec);
-
-
-      (*(* The others are declared as normal definitions *)
-      let var_subst id = (id, Constrintern.global_reference id) in
-      let _ = 
-	List.fold_left
-	  (fun subst (f,def,t) ->
-	     let ce = { const_entry_body = replace_vars subst def;
-			const_entry_type = Some t;
-			const_entry_opaque = false;
-			const_entry_boxed = boxed } in
-	     let _ =
-	       Declare.declare_constant f (DefinitionEntry ce,IsDefinition Definition)
-	     in
-      	       warning ((string_of_id f)^" is non-recursively defined");
-      	       (var_subst f) :: subst)
-	  (List.map var_subst (Array.to_list namerec))
-	  lnonrec 
-      in*)
-      List.iter (fun (df,c,scope) ->
-		   Metasyntax.add_notation_interpretation df [] c scope) notations
-  in 
-  let declare l = 
-    let recvec = Array.of_list l
-    and arrec = Array.map pi3 arrec
-    in declare arrec recvec
-  in
+    collect_non_rec env lrecnames recdef arityl nv in
   let recdefs = Array.length defrec in
-    trace (int recdefs ++ str " recursive definitions");
     (* Solve remaining evars *)
   let rec collect_evars i acc = 
     if i < recdefs then
       let (isevars, info, def) = defrec.(i) in
-      let _ = try trace (str "In solve evars, isevars is: " ++ Evd.pr_evar_defs !isevars) with _ -> () in
+	(*       let _ = try trace (str "In solve evars, isevars is: " ++ Evd.pr_evar_defs !isevars) with _ -> () in *)
       let def = evar_nf isevars def in
       let isevars = Evd.undefined_evars !isevars in
-      let _ = try trace (str "In solve evars, undefined is: " ++ Evd.pr_evar_defs isevars) with _ -> () in
+	(*       let _ = try trace (str "In solve evars, undefined is: " ++ Evd.pr_evar_defs isevars) with _ -> () in *)
       let evm = Evd.evars_of isevars in
       let _, _, typ = arrec.(i) in
       let id = namerec.(i) in
-      (* Generalize by the recursive prototypes  *)
+	(* Generalize by the recursive prototypes  *)
       let def = 
-	Termops.it_mkNamedLambda_or_LetIn def (Environ.named_context rec_sign)
+	Termops.it_mkNamedLambda_or_LetIn def rec_sign
       and typ = 
-	Termops.it_mkNamedProd_or_LetIn typ (Environ.named_context rec_sign) 
+	Termops.it_mkNamedProd_or_LetIn typ rec_sign
       in
-      let evars_def, evars_typ, evars = Eterm.eterm_term evm def (Some typ) in 	
-      (*let evars_typ = match evars_typ with Some t -> t | None -> assert(false) in*)
-      (*let fi = id_of_string (string_of_id id ^ "_evars") in*)
-      (*let ce = 
-	{ const_entry_body = evars_def; 
-	  const_entry_type = Some evars_typ;
-	  const_entry_opaque = false;
-	  const_entry_boxed = boxed} in
-      let kn = Declare.declare_constant fi (DefinitionEntry ce,IsDefinition Definition) in
-	definition_message fi;
-	trace (str (string_of_id fi) ++ str " is defined");*)
-	let evar_sum =
-	  if evars = [] then None
-	  else (
-	    (try trace (str "Building evars sum for : ");
-	       List.iter
-		 (fun (n, t) -> trace (str "Evar " ++ str (string_of_id n) ++ spc () ++ my_print_constr env0 t))
-		 evars;
-	     with _ -> ());
-	    let sum = Subtac_utils.build_dependent_sum evars in
-	      (try trace (str "Evars sum: " ++ my_print_constr env0 (snd sum));
-	       with _ -> ());
-	      Some sum)
-	in
-	  collect_evars (succ i) ((id, evars_def, evar_sum) :: acc)
+      let evars, def = Eterm.eterm_obligations id nc_len evm def (Some typ) in
+	collect_evars (succ i) ((id, def, typ, evars) :: acc)
     else acc
   in 
   let defs = collect_evars 0 [] in
-
-  (* Solve evars then create the definitions *)
-  let real_evars = 
-    filter_map (fun (id, kn, sum) ->
-		  match sum with Some (sumtac, sumg) -> Some (id, kn, sumg, sumtac) | None -> None)
-      defs
-  in
-    match real_evars with
-	[] -> declare (List.rev_map (fun (id, c, _) ->
-				   snd (decompose_lam_n recdefs c)) defs)
-      | l ->
-
-    Subtac_utils.and_tac real_evars
-      (fun f _ gr ->
-	 let _ = trace (str "Got a proof of: " ++ pr_global gr ++
-			str "type: " ++ my_print_constr (Global.env ()) (Global.type_of_global gr)) in
-	 let constant = match gr with Libnames.ConstRef c -> c
-	   | _ -> assert(false)
-	 in
-	   try
-	     (*let value = Environ.constant_value (Global.env ()) constant in*)
-	     let pis = f (mkConst constant) in
-	       (try (trace (str "Accessors: " ++
-			   List.fold_right (fun (_, _, _, c) acc -> my_print_constr env0 c ++ spc () ++ acc)
-			     pis (mt()));
-		    trace (str "Applied existentials: " ++
-			   (List.fold_right
-			      (fun (id, kn, sumg, pi) acc ->
-				 let args = Subtac_utils.destruct_ex pi sumg in
-				   my_print_constr env0 (mkApp (kn, Array.of_list args)))
-			      pis (mt ()))))
-	       with _ -> ());
-	       let rec aux pis acc = function
-		   (id, kn, sum) :: tl ->
-		     (match sum with 
-			  None -> aux pis (kn :: acc) tl
-			| Some (_, sumg) -> 
-			    let (id, kn, sumg, pi), pis = List.hd pis, List.tl pis in
-			    let args = Subtac_utils.destruct_ex pi sumg in
-			    let args = 
-			      List.map (fun c -> 
-					  try Reductionops.whd_betadeltaiota (Global.env ()) Evd.empty c
-					  with Not_found ->
-					    trace (str "Not_found while reducing " ++
-						   my_print_constr (Global.env ()) c);
-					    c
-				       ) args 				  
-			    in
-			    let _, newdef = decompose_lam_n (recdefs + List.length args) kn in
-			    let constr = Term.substl (mkRel 1 :: List.rev args) newdef in
-			      aux pis (constr :: acc) tl)
-		 | [] -> List.rev acc
-	       in
-		 declare (aux pis [] defs)
-	   with Environ.NotEvaluableConst cer ->
-	     match cer with
-		 Environ.NoBody -> trace (str "Constant has no body")
-	       | Environ.Opaque -> trace (str "Constant is opaque")
-      )
-*)
+    Subtac_obligations.add_mutual_definitions (List.rev defs) nvrec
+      
 let out_n = function
     Some n -> n
   | None -> 0
@@ -544,8 +405,7 @@ let build_recursive (lnameargsardef:(fixpoint_expr * decl_notation) list) boxed 
 		       errorlabstrm "Subtac_command.build_recursive"
 			 (str "Well-founded fixpoints not allowed in mutually recursive blocks"))
 	    lnameargsardef
-	in assert(false)
-	     (*build_mutrec lnameargsardef boxed*)
+	in build_mutrec lnameargsardef boxed
 	  
       
       
