contrib/subtac/Subtac.v
@@ -1,0 +1,2 @@
+Require Export Coq.subtac.Utils.
+Require Export Coq.subtac.FixSub.
